WellTyped.v
@@ -1,5 +1,5 @@
 Require Import Common.
-Require Import Syntax.
+Require Import Lang.
 Require Import List.
 
 
@@ -11,10 +11,13 @@ Module Ir.
 
 Definition dominates (from to:Ir.IRFunction.pc) (f:Ir.IRFunction.t) :=
   forall (exec:list Ir.IRFunction.pc)
+         (HLEN:List.length exec > 0)
+         (HBEGIN:List.hd from exec = Ir.IRFunction.get_begin_pc f)
+         (HEND:List.last exec to = to)
          (HVALID: forall_adj
                     (fun pc pc_next => Ir.IRFunction.valid_next_pc pc pc_next f)
-                    (exec ++ (to::nil)) = true),
-    List.In from (exec ++ (to::nil)).
+                    exec = true),
+    List.In from exec.
 
 (* Theorem: reflexivity of dominatedness. *)
 Theorem dominates_refl:
@@ -24,9 +27,24 @@ Proof.
   intros.
   unfold dominates.
   intros.
-  rewrite in_rev.
-  rewrite rev_unit.
-  constructor. reflexivity.
+  destruct exec.
+  simpl in HLEN. inversion HLEN.
+  simpl in HBEGIN.
+
+  apply last_head in HEND.
+  remember (rev (p::exec)) as l.
+  assert (List.length l = List.length (p::exec)).
+  { rewrite Heql. rewrite rev_length. reflexivity. }
+  destruct l.
+  - simpl in H. inversion H.
+  - simpl in HEND.
+    assert (p :: exec = rev (p0::l)).
+    { rewrite Heql. rewrite rev_involutive. reflexivity. }
+    rewrite H0.
+    apply in_rev. rewrite rev_involutive. rewrite HEND. constructor.
+    reflexivity.
+  - simpl.
+    apply Gt.gt_Sn_O.
 Qed.
 
 
